Challenge/Modexp/Submission/Proofs/Fast/Paths.lean
@@ -12,3 +12,4 @@ import Challenge.Modexp.Submission.Proofs.Fast.Paths.P10
 import Challenge.Modexp.Submission.Proofs.Fast.Paths.P11
 import Challenge.Modexp.Submission.Proofs.Fast.Paths.P12
 import Challenge.Modexp.Submission.Proofs.Fast.Paths.P13
+import Challenge.Modexp.Submission.Proofs.Fast.Paths.P14
